\documentclass{article}
\usepackage{epsfig}
\pagestyle{empty}
\begin{document}
$ xy $
\pagebreak

$ z $
\pagebreak

$ yz $
\pagebreak

$ x $
\pagebreak

$ zx $
\pagebreak

$ y $
\pagebreak

$ r_{inner}=0 $
\pagebreak

$ z$
\pagebreak

$ r_{inner}>0 $
\pagebreak

$ r = r_{outer} $
\pagebreak

$ r = r_{inner} $
\pagebreak

$ r_{inner}>0$
\pagebreak

$ \phi < \pi $
\pagebreak

$z$
\pagebreak

$ r = r_{outer}$
\pagebreak

$ \phi $
\pagebreak

$x$
\pagebreak

$ x$
\pagebreak

$y$
\pagebreak

$ \tan(\alpha) $
\pagebreak

$ z_min $
\pagebreak

$ z_max $
\pagebreak

$x^2 + y^2 = z^2 \tan \alpha$
\pagebreak

$\alpha$
\pagebreak

$t$
\pagebreak

$x_1$
\pagebreak

$x_2$
\pagebreak

$(x,y,z) = \vec x_1 + (\vec x_2 - \vec x_2) t $
\pagebreak

$(x,y,z)$
\pagebreak

$ \vec x_d = \frac{\vec x_2 - \vec x_1}{|\vec x_2 - \vec x_1|} $
\pagebreak

$t^2 (x_d^2 + y_d^2 - z_d^2 \tan^2 \alpha) + 2 t (x_1 x_d + y_1 y_d - z_1 z_d \tan^2 \alpha) + (x_1^2 + y_1^2 - z_1^2 \tan^2 \alpha) = 0 $
\pagebreak

$x_d$
\pagebreak

$ 2\cdot\phi_{half}$
\pagebreak

$ \phi_{ave} $
\pagebreak

$ d_0 $
\pagebreak

$ \vec d = \vec m - \vec c $
\pagebreak

$ \vec d $
\pagebreak

$ \vec{\texttt{measY}} = \vec{e}_z $
\pagebreak

$ \vec{\texttt{measX}} = \vec{\texttt{measY}} \times \frac{\vec{p}}{|\vec{p}|} $
\pagebreak

$ d_{0} $
\pagebreak

$ \vec{d} $
\pagebreak

$ \vec{measX} $
\pagebreak

$ sign = -sign(\vec{d} \cdot \vec{measX}) $
\pagebreak

$ \vec l_{a}(u) = \vec m_a + u \cdot \vec e_{a} $
\pagebreak

$ \vec l_{b}(\mu) = \vec m_b + \mu \cdot \vec e_{b} $
\pagebreak

$ \vec s(u, \mu) = \vec l_{b} - l_{a} = \vec m_{ab} + \mu \cdot \vec e_{b} - u \cdot \vec e_{a} $
\pagebreak

$ \vec m_{ab} = \vec m_{b} - \vec m_{a} $
\pagebreak

$ \vec s(u_0, \mu_0) $
\pagebreak

$ \vec l_{a,0} = l_{a}(u_0) $
\pagebreak

$ \vec l_{b,0} = l_{b}(\mu_0) $
\pagebreak

$ \vec e_{a} $
\pagebreak

$ \vec e_{b} $
\pagebreak

$ 0 = \vec s(u_0, \mu_0) \cdot \vec e_a = \vec m_{ab} \cdot \vec e_a + \mu_0 \vec e_a \cdot \vec e_b - u_0 $
\pagebreak

$ 0 = \vec s(u_0, \mu_0) \cdot \vec e_b = \vec m_{ab} \cdot \vec e_b + \mu_0 - u_0 \vec e_b \cdot \vec e_a $
\pagebreak

$ u $
\pagebreak

$ \mu_0 $
\pagebreak

$ u_0 = \frac{(\vec m_{ab} \cdot \vec e_a)-(\vec m_{ab} \cdot \vec e_b)(\vec e_a \cdot \vec e_b)}{1-(\vec e_a \cdot \vec e_b)^2} $
\pagebreak

$ \mu_0 = - \frac{(\vec m_{ab} \cdot \vec e_b)-(\vec m_{ab} \cdot \vec e_a)(\vec e_a \cdot \vec e_b)}{1-(\vec e_a \cdot \vec e_b)^2} $
\pagebreak

$ u_0 \simeq 0$
\pagebreak

$ u_0 $
\pagebreak

$ \vec n \cdot \vec x = \vec n \cdot \vec p,$
\pagebreak

$ \vec n = (n_{x}, n_{y}, n_{z})$
\pagebreak

$ \vec p = (p_{x}, p_{y}, p_{z})$
\pagebreak

$ \vec x = (x,y,z) $
\pagebreak

$ \vec l(u) = \vec l_{1} + u \cdot \vec v $
\pagebreak

$ u = \frac{\vec n (\vec p - \vec l_{1})}{\vec n \vec v}$
\pagebreak

$ eta $
\pagebreak

$ |x_{min}| $
\pagebreak

$ | x_{max} | $
\pagebreak

$ | y_{H} | $
\pagebreak

$ y = \kappa_{I} x + \delta_{I} $
\pagebreak

$ y = \kappa_{II} x + \delta_{II} $
\pagebreak

$ \kappa_{I} = - \kappa_{II} = 2 \frac{y_{H}}{x_{max} - x_{min}} $
\pagebreak

$ \delta_{I} = \delta_{II} = - \frac{1}{2}\kappa_{I}(x_{max} + x_{min}) $
\pagebreak

$[\text{xmin},\text{xmax})$
\pagebreak

$\text{nBins}$
\pagebreak

$l <= x < u$
\pagebreak

$1 \le \text{bin} \le \text{nBins} + 1$
\pagebreak

$0 \le \text{bin} \le \text{nBins}$
\pagebreak

$1 \le \text{bin} \le \text{nBins}$
\pagebreak

$\text{xmin} \le x < \text{xmax}$
\pagebreak

$\text{xmin_i} \le x_i < \text{xmax}_i \forall i=0, \dots, d-1$
\pagebreak

$2 \times \text{size}+1$
\pagebreak

$2^d$
\pagebreak

$d$
\pagebreak

$2^d = N $
\pagebreak

$ \alpha x^{2} + \beta x + \gamma = 0 $
\pagebreak

$ x_{1, 2} = - \frac{\beta \pm \sqrt{\beta^{2}-4\alpha\gamma}}{2\alpha}$
\pagebreak

$ \beta > 0 $
\pagebreak

$ x_{1} = - \frac{\beta + \sqrt{\beta^{2}-4\alpha\gamma}}{2\alpha} := \frac{q}{\alpha}$
\pagebreak

$ q= -\frac{1}{2}(\beta+sqrt{\beta^{2}-4\alpha\gamma})$
\pagebreak

$ x_{2} $
\pagebreak

$ x_{2} = \frac{\gamma}{q} = -\frac{2\gamma}{\beta+sqrt{\beta^{2}-4\alpha\gamma}}$
\pagebreak

$ -\frac{2\gamma}{\beta+sqrt{\beta^{2}-4\alpha\gamma}} = -\frac{2\gamma}{\beta}\frac{1}{1+\sqrt{1-4\alpha\gamma/\beta^{2}}}$
\pagebreak

$ x_{2}\frac{1}{1-\sqrt{1-4\alpha\gamma/\beta^{2}}} = -\frac{2\gamma}{\beta}\frac{1}{1-1+4\alpha\gamma/\beta^{2}}=-\frac{\beta}{2\alpha}.$
\pagebreak

$ -\frac{\beta(1-\sqrt{1-4\alpha\gamma/\beta^{2}}}{2\alpha} = - \frac{\beta - \sqrt{\beta^{2}-4\alpha\gamma}}{2\alpha} $
\pagebreak

$\text{lowerCorner}[i] \le \text{position}[i] \le \text{upperCorner}[i] \quad \forall i=0, \dots, d-1$
\pagebreak

$\mathcal{O}((|V| + |E|) log |V|)$
\pagebreak

$\ge 0$
\pagebreak

$\mathcal{O}(\mbox{length of this path})$
\pagebreak

$N$
\pagebreak

$\mathcal{O}(N)$
\pagebreak

$\mathcal{O}(E)$
\pagebreak

$E$
\pagebreak

$\mathcal{O}(1)$
\pagebreak

$ c = a + b $
\pagebreak

$ c = a * b $
\pagebreak

$ c = a / b $
\pagebreak

$M^2 = E^2 - p*p.$
\pagebreak

$"M^2" = E^2 - p^2 == M0^2 + Q^2 == M0^2 + t$
\pagebreak

$K_s^0$
\pagebreak

$\Lambda$
\pagebreak

$\overline{\Lambda}$
\pagebreak

$\gamma$
\pagebreak

$\chi^2_{prim}$
\pagebreak

$\chi^2_{geo}$
\pagebreak

$l/\Delta l$
\pagebreak

$\sigma_{M}$
\pagebreak

$\chi^2_{topo}$
\pagebreak

$K_s^0\rightarrow\pi^+\pi^-$
\pagebreak

$\Lambda\rightarrow p\pi^-$
\pagebreak

$\overline{\Lambda}\rightarrow \overline{p}\pi^+$
\pagebreak

$\gamma\rightarrow e^+e^-$
\pagebreak

$\pi^0\rightarrow \gamma\gamma$
\pagebreak

$\Xi^-\rightarrow \Lambda\pi^-$
\pagebreak

$\overline{\Xi}^-\rightarrow \overline{\Lambda}\pi^+$
\pagebreak

$\Omega^-\rightarrow \Lambda K^-$
\pagebreak

$\overline{\Omega}^-\rightarrow \overline{\Lambda} K^+$
\pagebreak

$\Xi$
\pagebreak

$\Omega$
\pagebreak

$J/\psi$
\pagebreak

$K^0_s$
\pagebreak

$\pi^0$
\pagebreak

$\Xi^-$
\pagebreak

$\overline{\Xi}^+$
\pagebreak

$\Omega^-$
\pagebreak

$\overline{\Omega}^+$
\pagebreak

$\Xi^{0*}$
\pagebreak

$\overline{\Xi}^{0*}$
\pagebreak

\end{document}
